bfn_fifo_3q_full.v
@@ -1,0 +1,224 @@
+(**************************************************************)
+(*   Copyright Dominique Larchey-Wendling [*]                 *)
+(*                                                            *)
+(*                             [*] Affiliation LORIA -- CNRS  *)
+(**************************************************************)
+(*      This file is distributed under the terms of the       *)
+(*         CeCILL v2 FREE SOFTWARE LICENSE AGREEMENT          *)
+(**************************************************************)
+
+(** Extraction of breadth-first numbering algorithm from Coq to Ocaml 
+
+       see http://okasaki.blogspot.com/2008/07/breadth-first-numbering-algorithm-in.html
+       and https://www.westpoint.edu/eecs/SiteAssets/SitePages/Faculty%20Publication%20Documents/Okasaki/jfp95queue.pdf
+       and https://www.cs.cmu.edu/~rwh/theses/okasaki.pdf
+       and https://www.westpoint.edu/eecs/SiteAssets/SitePages/Faculty%20Publication%20Documents/Okasaki/icfp00bfn.pdf
+
+*)
+
+Require Import List Arith Omega Extraction.
+Require Import list_utils wf_utils bt bft fifo.
+
+Set Implicit Arguments.
+
+Section seq_an.
+
+  (* seq_an a n = [a;a+1;...;a+(n-1)] *)
+
+  Fixpoint seq_an a n : list nat :=
+    match n with
+      | 0    => nil
+      | S n  => a::seq_an (S a) n
+    end.
+
+  Fact seq_an_length a n : length (seq_an a n) = n.
+  Proof. revert a; induction n; simpl; intros; f_equal; auto. Qed.
+
+  Fact seq_an_spec a n x : In x (seq_an a n) <-> a <= x < a+n.
+  Proof. 
+    revert x a; induction n as [ | n IHn ]; intros x a; simpl;
+      [ | rewrite IHn ]; omega.
+  Qed.
+
+  Fixpoint is_seq_from n (l : list nat) { struct l }: Prop :=
+    match l with  
+      | nil  => True
+      | x::l => n = x /\ is_seq_from (S n) l
+    end.
+
+  Theorem is_seq_from_spec a l : is_seq_from a l <-> exists n, l = seq_an a n.
+  Proof.
+    revert a; induction l as [ | x l IH ]; intros a; simpl.
+    + split; auto; exists 0; auto.
+    + rewrite IH; split.
+      * intros (? & n & Hn); subst x; exists (S n); subst; auto.
+      * intros ([ | n ] & ?); subst; try discriminate.
+        simpl in H; inversion H; subst; split; auto.
+        exists n; auto.
+  Qed.
+
+End seq_an.
+
+Section bfn.
+
+  Let fifo_3q_sum { X } (q : fifo_3q (bt X)) := lsum (fifo_3q_list q). 
+
+  Variable (X : Type).
+
+  Notation fX := (fifo_3q (bt X)). 
+  Notation fN := (fifo_3q (bt nat)).
+
+  (* the forest (list of bt nat) is a breadth first numbering from n if
+     its breadth first traversal yields [n;n+1;....;m[ for some m
+   *)
+
+(*
+  Let fX_spec := fifo_3q_spec (bt X).
+  Let fN_spec := fifo_3q_spec (bt nat).
+
+*)
+
+  Definition is_bfn_from n l := is_seq_from n (bft_f l).
+
+  (* Breath First Numbering: maps a forest X to a forest nat such that
+          1) the two forests are of the same shape
+          2) the result is a breadth first numbering from n
+
+     Beware that the output is a reversed queue compared to the input
+   *)
+
+  (** The structure of this proof is the following:
+
+      We use refine to specify the computational content and
+      proof obligations are solved inside { }.
+
+      At some point, we need pattern matching to decompose 
+      term in hypotheses as well as in the conclusion. The
+      simplest way to do it is to revert the hypothesis in 
+      the conclusion before the match and intro it in the
+      different match branches. This corresponds to dependent
+      pattern matching but hand-writting it in refines is
+      much more complicated than
+
+      revert Hq; refine (match q with ... => ... end); intros Hq
+
+      By solving proof obligations in {}, we let the computational 
+      content to develop itself in the main branch
+
+      Also, using fully specified terms fifo_3q_*_full also
+      use to avoid generalizing fifo_3q_*_spec before the
+      next pattern matching
+
+    *)
+
+  Definition bfn_3q_f n (p : fX) : { q : fN | fifo_3q_list p ~lt rev (fifo_3q_list q) /\ is_bfn_from n (rev (fifo_3q_list q)) }.
+  Proof.
+    induction on n p as bfn_3q_f with measure (fifo_3q_sum p).
+
+    refine (let (b,Hb) := fifo_3q_void_full p in _);
+    revert Hb; refine (match b with 
+      | true  => fun Hp => exist _ fifo_3q_nil _
+      | false => fun Hp => let (d1,Hd1) := fifo_3q_deq_full p _ in _
+    end).
+ 
+    { apply proj1 in Hp; rewrite Hp, fifo_3q_nil_spec; split; simpl; auto.
+      red; rewrite bft_f_fix_0; simpl; auto. }
+    { intros H; apply Hp in H; discriminate. }
+
+    revert Hd1; refine (match d1 with
+      | (leaf x    , p1) => fun Hp1 => let (q,Hq) := bfn_3q_f (S n) p1 _ 
+                                       in  exist _ (fifo_3q_enq q (leaf n)) _
+      | (node a x b, p1) => fun Hp1 => let (q,Hq) := bfn_3q_f (S n) (fifo_3q_enq (fifo_3q_enq p1 a) b) _ in 
+                                       let (d2,Hd2) := fifo_3q_deq_full q _ 
+                                       in  _
+    end); simpl in Hp1.
+
+    { unfold fifo_3q_sum; rewrite Hp1; simpl; omega. }
+    { destruct Hq as (H5 & H6).
+      rewrite Hp1, fifo_3q_enq_spec.
+      subst; split; auto.
+      + rewrite rev_app_distr; simpl; auto.
+      + rewrite rev_app_distr; simpl; red.
+        rewrite bft_f_fix_3; simpl; rewrite <- app_nil_end; auto. }
+    { unfold fifo_3q_sum. 
+      rewrite fifo_3q_enq_spec, fifo_3q_enq_spec, app_ass; simpl.
+      rewrite lsum_app, Hp1; simpl; omega. }
+    { apply proj1, Forall2_rev in Hq; intros H; revert Hq.
+      rewrite H, fifo_3q_enq_spec, fifo_3q_enq_spec, app_ass; simpl.
+      rewrite rev_app_distr; inversion 1. }
+
+    revert Hd2; refine (match d2 with (u,q1) => _ end); intros Hq1;
+    refine (let (d3,Hd3) := fifo_3q_deq_full q1 _ in _).
+
+    { apply proj1, Forall2_rev in Hq; intros H; revert Hq.
+      rewrite Hq1, H, fifo_3q_enq_spec, fifo_3q_enq_spec, app_ass; simpl.
+      rewrite rev_app_distr; simpl. 
+      inversion 1; inversion H6. }
+
+    revert Hd3; refine (match d3 with 
+      | (v,q2) => fun Hq2 => let (q3,Hq3) := fifo_3q_enq_full q2 (node v n u)
+                             in  exist _ q3 _
+    end); simpl in Hq2, Hq3.
+
+    { destruct Hq as (H5,H6).
+      rewrite fifo_3q_enq_spec, fifo_3q_enq_spec, Hq1, Hq2 in H5. 
+      repeat (rewrite app_ass in H5; simpl in H5).
+      apply Forall2_2snoc_inv in H5.
+      destruct H5 as (G1 & G2 & H5).
+      rewrite Hq1, Hq2 in H6; simpl in H6; rewrite app_ass in H6; simpl in H6.
+      unfold is_bfn_from in H6 |- *.
+      rewrite Hp1, Hq3, rev_app_distr; simpl.  
+      rewrite bft_f_fix_3; simpl; split; auto. }
+  Defined.
+
+  Section bfn.
+
+    Let bfn_3q_full (t : bt X) : { t' | t ~t t' /\ is_seq_from 0 (bft_std t') }.
+    Proof.
+      refine (match @bfn_3q_f 0 (fifo_3q_enq fifo_3q_nil t) with 
+        | exist _ q Hq => let (d1,Hd1) := fifo_3q_deq_full q _ in _ 
+      end).
+
+      { intros H; rewrite fifo_3q_enq_spec, fifo_3q_nil_spec, H in Hq.
+        apply proj1 in Hq; inversion Hq. }
+
+      revert Hd1; refine (match d1 with (x,q1) => fun Hq1 => exist _ x _ end); simpl in Hq1.
+
+      { rewrite fifo_3q_enq_spec, fifo_3q_nil_spec in Hq; destruct Hq as (H1 & H2).
+        rewrite <- bft_std_eq_bft.
+        rewrite Hq1 in H1; simpl in H1.
+        apply Forall2_snoc_inv with (l := nil) in H1.
+        destruct H1 as (G1 & H1).
+        apply Forall2_nil_inv_right in H1.
+        apply f_equal with (f := @rev _) in H1.
+        rewrite rev_involutive in H1; simpl in H1.
+        rewrite Hq1, H1 in H2; simpl in H2.
+        auto. }
+    Qed.
+
+    Definition bfn_3q t := proj1_sig (bfn_3q_full t).
+
+    Fact bfn_3q_spec_1 t : t ~t bfn_3q t.
+    Proof. apply (proj2_sig (bfn_3q_full t)). Qed.
+
+    Fact bfn_3q_spec_2 t : exists n, bft_std (bfn_3q t) = seq_an 0 n.
+    Proof. apply is_seq_from_spec, (proj2_sig (bfn_3q_full t)). Qed.
+
+  End bfn.
+
+End bfn.
+
+(* Notice that fifo_3q_deq is extracted to a function that loops forever
+   if the input is the empty queue, ie does not following the spec *)
+
+Extract Inductive bool => "bool" [ "true" "false" ].
+Extract Inductive prod => "(*)"  [ "(,)" ].
+Extract Inductive nat => int [ "0" "succ" ] "(fun fO fS n -> if n=0 then fO () else fS (n-1))".
+
+Recursive Extraction bfn_3q.
+
+Check bfn_3q.
+Check bfn_3q_spec_1.
+Check bfn_3q_spec_2.
+             
+
